code/bignum/Hacl.Bignum.Lib.fst
@@ -148,39 +148,42 @@ let bn_get_top_index #t =
 
 
 inline_for_extraction noextract
+val bn_get_bits_limb:
+    #t:limb_t
+  -> len:size_t
+  -> n:lbignum t len
+  -> ind:size_t{v ind / bits t < v len} ->
+  Stack (limb t)
+  (requires fun h -> live h n)
+  (ensures  fun h0 r h1 -> modifies0 h0 h1 /\
+    r == S.bn_get_bits_limb (as_seq h0 n) (v ind))
+
+let bn_get_bits_limb #t len n ind =
+  [@inline_let]
+  let pbits = size (bits t) in
+  let i = ind /. pbits in
+  assert (v i == v ind / bits t);
+  let j = ind %. pbits in
+  assert (v j == v ind % bits t);
+  let p1 = n.(i) >>. j in
+  if i +! 1ul <. len && 0ul <. j then
+    p1 |. (n.(i +! 1ul) <<. (pbits -! j))
+  else
+    p1
+
+
+inline_for_extraction noextract
 val bn_get_bits:
     #t:limb_t
   -> len:size_t
   -> b:lbignum t len
   -> i:size_t
-  -> l:size_t{v l <= bits t /\ (v i + v l - 1) / bits t < v len /\ v i + v l <= max_size_t} ->
+  -> l:size_t{v l < bits t /\ v i / bits t < v len} ->
   Stack (limb t)
   (requires fun h -> live h b)
   (ensures  fun h0 r h1 -> modifies0 h0 h1 /\
     r == S.bn_get_bits (as_seq h0 b) (v i) (v l))
 
 let bn_get_bits #t len b i l =
-  push_frame ();
-  let acc = create 1ul (uint #t 0) in
-
-  let h0 = ST.get () in
-  [@ inline_let]
-  let refl h i = LSeq.index (as_seq h acc) 0 in
-  [@ inline_let]
-  let spec h0 = S.bn_get_bits_f (as_seq h0 b) (v i) (v l) in
-
-  [@ inline_let]
-  let inv h (i:nat{i <= v l}) =
-    modifies1 acc h0 h /\
-    live h acc /\ live h b /\ disjoint acc b /\
-    refl h i == Loops.repeati i (spec h0) (refl h0 0) in
-
-  Loops.eq_repeati0 (v l) (spec h0) (refl h0 0);
-  Lib.Loops.for 0ul l inv
-  (fun j ->
-    Loops.unfold_repeati (v l) (spec h0) (refl h0 0) (v j);
-    let b_ij = bn_get_ith_bit len b (i +! j) in
-    acc.(0ul) <- acc.(0ul) +. (b_ij <<. j));
-  let res = acc.(0ul) in
-  pop_frame ();
-  res
+  let mask_l = (uint #t #SEC 1 <<. l) -. uint #t 1 in
+  bn_get_bits_limb len b i &. mask_l
